about to use wind for everything

basic_types.v
@@ -5,9 +5,6 @@ From istari Require Import Sigma Tactics
      Syntax Subst SimpSub Promote Hygiene
      ContextHygiene Equivalence Rules Defined.
 
-
-
-
 Definition oof M A: (@Syntax.judgement obj) := deq M M A.
 
 Definition oof_t M: (@Syntax.judgement obj) := deqtype M M.
@@ -49,4 +46,96 @@ Lemma U0_type: forall G,
 
 Hint Resolve nat_type nat_U0 zero_typed leq_refl leq_type lt_type U0_type.
 
+Definition if_z (n: term obj): (term obj) := ppi1 n.
 
+(*n - m*)
+Definition minusbc: (term obj) := lam
+                         (
+                           (*f := 0*)
+                           lam ( (*f:= 1, n := 0*)
+                               lam ((*f := 2, n:= 1, m := 0*)
+                                   let f := (var 2) in
+                                   let n := (var 1) in
+                                   let m := (var 0) in
+                                                  bite (if_z n)
+                                                  (n)
+                                                  (bite (if_z m)
+                                                     (n)
+                                                    (app (app f (app (ppi2 n) triv)) (app (ppi2 m) triv)))
+                                                  ))).
+ Definition minus: (term obj) := app theta minusbc.
+
+ Lemma minus_typed {G}: tr G (oof minus (arrow nattp (arrow nattp nattp))).
+Admitted.
+
+(*lt_b x y*)
+ Definition lt_b := lam ( lam (*x = 1, y = 0*)
+
+                            (if_z (app (app minus (nsucc (var 1)))  (var 0)))
+                       ).
+
+Definition ltb_app m n := app (app lt_b m) n.
+
+(*should be fine*)
+Lemma ltapp_typed G m n: tr G (oof m nattp) -> tr G (oof n nattp) ->
+  tr G (oof (ltb_app m n) booltp). Admitted.
+
+(*more difficult, need induction*)
+Lemma ltb_false G n : tr G (oof n nattp) -> tr G (deq (ltb_app n n) bfalse booltp).
+Admitted.
+
+Lemma nsucc_lt: forall G n, tr G (oof n nattp) ->
+                       tr G (oof triv (lt_t n (nsucc n))).
+Admitted.
+
+
+Definition eq_bbc: (term obj) := lam
+                         (
+                           (*f := 0*)
+                           lam ( (*f:= 1, n := 0*)
+                               lam ((*f := 2, n:= 1, m := 0*)
+                                   let f := (var 2) in
+                                   let n := (var 1) in
+                                   let m := (var 0) in
+                                                  bite (if_z n)
+                                                  (if_z m)
+                                                  (bite (if_z m)
+                                                     (bfalse)
+                                                    (app (app f (app (ppi2 n) triv)) (app (ppi2 m) triv)))
+                                                  ))).
+ Definition eq_b: (term obj) := app theta eq_bbc.
+
+Lemma eqb_typed {G}: tr G (oof eq_b (arrow nattp (arrow nattp booltp))).
+Admitted.
+
+Lemma eqapp_typed G m n: tr G (oof m nattp) -> tr G (oof n nattp) ->
+  tr G (oof (app (app eq_b m) n) booltp). Admitted.
+
+Lemma eqb_P G n m : tr G (oof n nattp) ->
+                    tr G (oof m nattp) ->
+  tr G (deq (app (app eq_b n) m) btrue booltp) ->
+                    tr G (deq n m nattp).
+  intros.
+Admitted.
+
+
+Definition eq_wind = wind (lam (* x = 0*)
+                             (lam (*x = 1, y= 0*)
+                                ( lam
+                                    ( (*x = 2, y = 1, z = 0*)
+                                      bite x
+                                           (lam (*x = 3, y = 2, z = 1, n2 = 0*)
+                                              (if_z (var 0))
+                                           ) (*first one is zero*)
+                                           ( (*first one is nonzero*)
+                                             lam
+                                               ( (*x = 3, y = 2, z = 1, n2 = 0*)
+                                                 bite (if_z (var 0))
+                                                      false
+                                                      (z * (ppi2 (var 0)) *)
+                                               )
+                                           )
+                                    )
+                                )
+                             )                           
+                          )
